wip

ems/Skeleton.v
@@ -46,7 +46,7 @@ Qed.
 
 Module SkEnv.
 
-  Notation mblock := nat (only parsing).
+  Notation mblock := positive (only parsing).
   Notation ptrofs := Z (only parsing).
 
   Record t: Type := mk {
@@ -158,136 +158,146 @@ Module Sk.
   (*** TODO: It might be nice if Sk.t also constitutes a resource algebra ***)
   (*** At the moment, List.app is not assoc/commutative. We need to equip RA with custom equiv. ***)
 
+  Definition pos2nat := fun blk => (Pos.to_nat blk) - 1.
+  Definition nat2pos := Pos.of_succ_nat.
+
+  Lemma nat2pos_pos2nat_id : forall n, pos2nat (nat2pos n) = n.
+  Proof. i. unfold pos2nat, nat2pos. nia. Qed.
+  
+  Lemma pos2nat_nat2pos_id : forall p, nat2pos (pos2nat p) = p.
+  Proof. i. unfold pos2nat, nat2pos. nia. Qed.
+    
+
   Definition load_skenv (sk: t): (SkEnv.t) :=
     let n := List.length sk in
     {|
-      SkEnv.blk2id := fun blk => do '(gn, _) <- (List.nth_error sk blk); Some gn;
-      SkEnv.id2blk := fun id => do '(blk, _) <- find_idx (fun '(id', _) => string_dec id id') sk; Some blk
+      SkEnv.blk2id := fun blk => do '(gn, _) <- (List.nth_error sk (pos2nat blk) ); Some gn;
+      SkEnv.id2blk := fun id => do '(idx, _) <- find_idx (fun '(id', _) => string_dec id id') sk; Some (nat2pos idx) 
     |}
   .
 
-  Lemma load_skenv_wf
-        sk
-        (WF: wf sk)
-    :
-      <<WF: SkEnv.wf (load_skenv sk)>>
-  .
-  Proof.
-    r in WF.
-    rr. split; i; ss.
-    - uo; des_ifs.
-      + f_equal. ginduction sk; ss. i. inv WF.
-        rewrite find_idx_red in Heq1. des_ifs; ss.
-        { des_sumbool. subst. ss. clarify. }
-        des_sumbool. uo. des_ifs. destruct p. ss.
-        hexploit IHsk; et.
-      + exfalso. ginduction sk; ss. i. inv WF.
-        rewrite find_idx_red in Heq2. des_ifs; ss.
-        des_sumbool. uo. des_ifs. destruct p. ss.
-        hexploit IHsk; et.
-    - ginduction sk; ss.
-      { i. uo. ss. destruct blk; ss. }
-      i. destruct a. inv WF. uo. destruct blk; ss; clarify.
-      {  rewrite find_idx_red. uo. des_ifs; des_sumbool; ss. }
-      hexploit IHsk; et. i.
-      rewrite find_idx_red. uo. des_ifs; des_sumbool; ss. exfalso.
-      subst. clear - Heq1 H2. ginduction sk; ss. i.
-      rewrite find_idx_red in Heq1. des_ifs; des_sumbool; ss; et.
-      uo. des_ifs. destruct p. eapply IHsk; et.
-  Qed.
+  (* Lemma load_skenv_wf *)
+  (*       sk *)
+  (*       (WF: wf sk) *)
+  (*   : *)
+  (*     <<WF: SkEnv.wf (load_skenv sk)>> *)
+  (* . *)
+  (* Proof. *)
+  (*   r in WF. *)
+  (*   rr. split; i; ss. *)
+  (*   - uo; des_ifs. *)
+  (*     + f_equal. ginduction sk; ss. i. inv WF. *)
+  (*       rewrite find_idx_red in Heq1. des_ifs; ss. *)
+  (*       { des_sumbool. subst. ss. clarify. } *)
+  (*       des_sumbool. uo. des_ifs. destruct p. ss. *)
+  (*       hexploit IHsk; et. *)
+  (*     + exfalso. ginduction sk; ss. i. inv WF. *)
+  (*       rewrite find_idx_red in Heq2. des_ifs; ss. *)
+  (*       des_sumbool. uo. des_ifs. destruct p. ss. *)
+  (*       hexploit IHsk; et. *)
+  (*   - ginduction sk; ss. *)
+  (*     { i. uo. ss. destruct blk; ss. } *)
+  (*     i. destruct a. inv WF. uo. destruct blk; ss; clarify. *)
+  (*     {  rewrite find_idx_red. uo. des_ifs; des_sumbool; ss. } *)
+  (*     hexploit IHsk; et. i. *)
+  (*     rewrite find_idx_red. uo. des_ifs; des_sumbool; ss. exfalso. *)
+  (*     subst. clear - Heq1 H2. ginduction sk; ss. i. *)
+  (*     rewrite find_idx_red in Heq1. des_ifs; des_sumbool; ss; et. *)
+  (*     uo. des_ifs. destruct p. eapply IHsk; et. *)
+  (* Qed. *)
 
-  Definition incl (sk0 sk1: Sk.t): Prop :=
-    forall gn gd (IN: List.In (gn, gd) sk0),
-      List.In (gn, gd) sk1.
+  (* Definition incl (sk0 sk1: Sk.t): Prop := *)
+  (*   forall gn gd (IN: List.In (gn, gd) sk0), *)
+  (*     List.In (gn, gd) sk1. *)
 
-  Program Instance incl_PreOrder: PreOrder incl.
-  Next Obligation.
-  Proof.
-    ii. ss.
-  Qed.
-  Next Obligation.
-  Proof.
-    ii. eapply H0. eapply H. ss.
-  Qed.
+  (* Program Instance incl_PreOrder: PreOrder incl. *)
+  (* Next Obligation. *)
+  (* Proof. *)
+  (*   ii. ss. *)
+  (* Qed. *)
+  (* Next Obligation. *)
+  (* Proof. *)
+  (*   ii. eapply H0. eapply H. ss. *)
+  (* Qed. *)
 
-  Lemma sort_incl sk
-    :
-      incl sk (sort sk).
-  Proof.
-    ii. eapply Permutation.Permutation_in; [|apply IN].
-    eapply SkSort.sort_permutation.
-  Qed.
+  (* Lemma sort_incl sk *)
+  (*   : *)
+  (*     incl sk (sort sk). *)
+  (* Proof. *)
+  (*   ii. eapply Permutation.Permutation_in; [|apply IN]. *)
+  (*   eapply SkSort.sort_permutation. *)
+  (* Qed. *)
 
-  Lemma sort_incl_rev sk
-    :
-      incl (sort sk) sk.
-  Proof.
-    ii. eapply Permutation.Permutation_in; [|apply IN].
-    symmetry. eapply SkSort.sort_permutation.
-  Qed.
+  (* Lemma sort_incl_rev sk *)
+  (*   : *)
+  (*     incl (sort sk) sk. *)
+  (* Proof. *)
+  (*   ii. eapply Permutation.Permutation_in; [|apply IN]. *)
+  (*   symmetry. eapply SkSort.sort_permutation. *)
+  (* Qed. *)
 
-  Definition incl_env (sk0: Sk.t) (skenv: SkEnv.t): Prop :=
-    forall gn gd (IN: List.In (gn, gd) sk0),
-    exists blk, <<FIND: skenv.(SkEnv.id2blk) gn = Some blk>>.
+  (* Definition incl_env (sk0: Sk.t) (skenv: SkEnv.t): Prop := *)
+  (*   forall gn gd (IN: List.In (gn, gd) sk0), *)
+  (*   exists blk, <<FIND: skenv.(SkEnv.id2blk) gn = Some blk>>. *)
 
-  Lemma incl_incl_env sk0 sk1
-        (INCL: incl sk0 sk1)
-    :
-      incl_env sk0 (load_skenv sk1).
-  Proof.
-    ii. exploit INCL; et. i. ss. uo. des_ifs; et.
-    exfalso. clear - x0 Heq0. ginduction sk1; et.
-    i. ss. rewrite find_idx_red in Heq0. des_ifs.
-    des_sumbool. uo.  des_ifs. des; clarify.
-    eapply IHsk1; et.
-  Qed.
+  (* Lemma incl_incl_env sk0 sk1 *)
+  (*       (INCL: incl sk0 sk1) *)
+  (*   : *)
+  (*     incl_env sk0 (load_skenv sk1). *)
+  (* Proof. *)
+  (*   ii. exploit INCL; et. i. ss. uo. des_ifs; et. *)
+  (*   exfalso. clear - x0 Heq0. ginduction sk1; et. *)
+  (*   i. ss. rewrite find_idx_red in Heq0. des_ifs. *)
+  (*   des_sumbool. uo.  des_ifs. des; clarify. *)
+  (*   eapply IHsk1; et. *)
+  (* Qed. *)
 
-  Lemma in_env_in_sk :
-    forall sk blk symb
-      (FIND: SkEnv.blk2id (Sk.load_skenv sk) blk = Some symb),
-    exists def, In (symb, def) sk.
-  Proof.
-    i. unfold SkEnv.blk2id. ss.
-    uo. des_ifs. des; clarify.
-    eapply nth_error_In in Heq0. et.
-  Qed.
+  (* Lemma in_env_in_sk : *)
+  (*   forall sk blk symb *)
+  (*     (FIND: SkEnv.blk2id (Sk.load_skenv sk) blk = Some symb), *)
+  (*   exists def, In (symb, def) sk. *)
+  (* Proof. *)
+  (*   i. unfold SkEnv.blk2id. ss. *)
+  (*   uo. des_ifs. des; clarify. *)
+  (*   eapply nth_error_In in Heq0. et. *)
+  (* Qed. *)
 
-  Lemma in_sk_in_env :
-    forall sk def symb
-           (IN: In (symb, def) sk),
-    exists blk, SkEnv.blk2id (Sk.load_skenv sk) blk = Some symb.
-  Proof.
-    i. unfold SkEnv.blk2id. ss.
-    uo. eapply In_nth_error in IN. des.
-    eexists. rewrite IN. et.
-  Qed.
+  (* Lemma in_sk_in_env : *)
+  (*   forall sk def symb *)
+  (*          (IN: In (symb, def) sk), *)
+  (*   exists blk, SkEnv.blk2id (Sk.load_skenv sk) blk = Some symb. *)
+  (* Proof. *)
+  (*   i. unfold SkEnv.blk2id. ss. *)
+  (*   uo. eapply In_nth_error in IN. des. *)
+  (*   eexists. rewrite IN. et. *)
+  (* Qed. *)
 
-  Lemma env_range_some :
-    forall sk blk
-      (BLKRANGE : blk < Datatypes.length sk),
-      <<FOUND : exists symb, SkEnv.blk2id (Sk.load_skenv sk) blk = Some symb>>.
-  Proof.
-    i. depgen sk. induction blk; i; ss; clarify.
-    { destruct sk; ss; clarify.
-      { lia. }
-      uo. destruct p. exists s. ss. }
-    destruct sk; ss; clarify.
-    { lia. }
-    apply lt_S_n in BLKRANGE. eapply IHblk; eauto.
-  Qed.
+  (* Lemma env_range_some : *)
+  (*   forall sk blk *)
+  (*     (BLKRANGE : blk < Datatypes.length sk), *)
+  (*     <<FOUND : exists symb, SkEnv.blk2id (Sk.load_skenv sk) blk = Some symb>>. *)
+  (* Proof. *)
+  (*   i. depgen sk. induction blk; i; ss; clarify. *)
+  (*   { destruct sk; ss; clarify. *)
+  (*     { lia. } *)
+  (*     uo. destruct p. exists s. ss. } *)
+  (*   destruct sk; ss; clarify. *)
+  (*   { lia. } *)
+  (*   apply lt_S_n in BLKRANGE. eapply IHblk; eauto. *)
+  (* Qed. *)
 
-  Lemma env_found_range :
-    forall sk symb blk
-      (FOUND : SkEnv.id2blk (Sk.load_skenv sk) symb = Some blk),
-      <<BLKRANGE : blk < Datatypes.length sk>>.
-  Proof.
-    induction sk; i; ss; clarify.
-    uo; des_ifs. destruct p0. rewrite find_idx_red in Heq0. des_ifs.
-    { apply Nat.lt_0_succ. }
-    destruct blk.
-    { apply Nat.lt_0_succ. }
-    uo. des_ifs. destruct p. ss. clarify. apply lt_n_S. eapply IHsk; eauto.
-    instantiate (1:=symb). rewrite Heq0. ss.
-  Qed.
+  (* Lemma env_found_range : *)
+  (*   forall sk symb blk *)
+  (*     (FOUND : SkEnv.id2blk (Sk.load_skenv sk) symb = Some blk), *)
+  (*     <<BLKRANGE : blk < Datatypes.length sk>>. *)
+  (* Proof. *)
+  (*   induction sk; i; ss; clarify. *)
+  (*   uo; des_ifs. destruct p0. rewrite find_idx_red in Heq0. des_ifs. *)
+  (*   { apply Nat.lt_0_succ. } *)
+  (*   destruct blk. *)
+  (*   { apply Nat.lt_0_succ. } *)
+  (*   uo. des_ifs. destruct p. ss. clarify. apply lt_n_S. eapply IHsk; eauto. *)
+  (*   instantiate (1:=symb). rewrite Heq0. ss. *)
+  (* Qed. *)
 
 End Sk.
